End of day 17/07/18

michael_formal/Trace_LTL.thy
@@ -22,11 +22,52 @@ inductive Until :: "efsm \<Rightarrow> statename \<Rightarrow> datastate \<Right
   until_h: "f' s d p (shd t) \<Longrightarrow> Until e s d p t f f'" |
   until_t: "f s d p (shd t) \<Longrightarrow> step e s d (fst (shd t)) (snd (shd t)) = Some (s', o', d') \<and> Until e s' d' o' (stl t) f f' \<Longrightarrow> Until e s d p t f f'"
 
-lemma "Until filesystem 1 <> [] t (\<lambda>s d p (l, i). s = 1) (\<lambda>s d p (l, i). l=''login'')"
-proof (induction t)
-case (1 y)
+coinductive valid_trace_aux :: "efsm \<Rightarrow> statename \<Rightarrow> datastate \<Rightarrow> event stream \<Rightarrow> bool" where
+  C_always: "step e s d (fst (shd t)) (snd (shd t)) = Some (s', o', d') \<Longrightarrow> valid_trace_aux e s' d' (stl t) \<Longrightarrow> valid_trace_aux e s d t"
+
+abbreviation valid_trace :: "efsm \<Rightarrow> event stream \<Rightarrow> bool" where
+  "valid_trace e t \<equiv> valid_trace_aux e (s0 e) <> t"
+
+lemma valid_first_step: "valid_trace e t \<Longrightarrow> step e (s0 e) <> (fst (shd t)) (snd (shd t)) \<noteq> None"
+  apply simp
+  apply (rule ccontr)
+  apply simp
+  by (meson valid_trace_aux.cases)
+
+lemma valid_step: "valid_trace_aux e s d t \<Longrightarrow> step e s d (fst (shd t)) (snd (shd t)) \<noteq> None"
+  apply simp
+  apply (rule ccontr)
+  apply simp
+  using valid_trace_aux.simps by blast
+
+lemma invalid_step: "step e s d (fst (shd t)) (snd (shd t)) = None \<Longrightarrow> \<not> valid_trace_aux e s d t"
+  using valid_step by blast
+
+lemma login_wrong_arity: "\<not> (fst (shd t) = ''login'' \<and> length (snd (shd t)) = Suc 0) \<Longrightarrow> step filesystem 1 <> (fst (shd t)) (snd (shd t)) = None"
+  by (simp add: step_def fs_simp)
+
+lemma "fst (shd t) = ''login'' \<longrightarrow> length (snd (shd t)) \<noteq> Suc 0 \<Longrightarrow> \<not> valid_trace_aux filesystem 1 Map.empty t"
+  apply (rule ccontr)
+  apply simp
+  
+
+
+lemma "valid_trace_aux filesystem 1 Map.empty t \<Longrightarrow> fst (shd t) = ''login'' \<and> length (snd (shd t)) = 1"
+  apply simp
+  apply (rule ccontr)
+  apply simp
+
+
+lemma "valid_trace filesystem t \<Longrightarrow> globally filesystem 1 <> [] t (\<lambda>s d p e. s = 1 \<or> s = 2)"
+proof (coinduction)
+case globally
   then show ?case
-apply simp
+    apply simp
+    apply (rule_tac x=2 in exI)
+    apply (rule_tac x="[]" in exI)
+    apply (rule_tac x="<R 1 := hd (snd (shd t))>" in exI)
+    apply simp
+    apply safe
 qed
   
 end
